lean/Governance/vendor/workspace/nalgebra/src/third_party/glam/mod.rs
@@ -1,8 +1,0 @@
-#[cfg(feature = "glam030")]
-mod v030;
-#[cfg(feature = "glam031")]
-mod v031;
-#[cfg(feature = "glam032")]
-mod v032;
-#[cfg(feature = "glam033")]
-mod v033;
